preservation.lean
@@ -92,422 +92,31 @@ lemma same_free_and_left {P P' Q: prop}: FV P' = FV P → (FV (P' ⋀ Q) = FV (P
     )
   )
 
-lemma dominates_self: ∀ {P: prop} {σ: env}, dominates σ P P
-| P σ :=
-  show dominates σ P P, from dominates_of (
-    assume h_impl: σ ⊨ P.instantiated_p,
-    have h_calls: calls_p_subst σ P ⊆ calls_p_subst σ P, from set.subset.refl (calls_p_subst σ P),
-    have h_quantifiers_p:
-      (∀(t': term) (x: var) (Q₁: prop) (h: callquantifier.mk t' x Q₁ ∈ quantifiers_p P),
-                            have Q₁.size < P.size, from quantifiers_smaller_than_prop.left h,
-      ∃(t: term) (Q₂: prop), callquantifier.mk t x Q₂ ∈ quantifiers_p P ∧
-                            (∀v: value, dominates' Q₁ Q₂ (σ[x↦v]))), from (
-      assume (t₁: term) (x:var) (Q₁: prop),
-      assume h2: callquantifier.mk t₁ x Q₁ ∈ quantifiers_p P,
-      have Q₁.size < P.size, from quantifiers_smaller_than_prop.left h2,
-      have (∀v: value, dominates' Q₁ Q₁ (σ[x↦v])), from (
-        assume v: value,
-        dominates_self
-      ),
-      exists.intro t₁ (exists.intro Q₁ ⟨h2, this⟩)
-    ),
-    ⟨h_impl, ⟨h_calls, h_quantifiers_p⟩⟩
-  )
-
-lemma dominates_and_left {P P' Q: prop} {σ: env}:
-      dominates σ P' P → dominates σ (P' ⋀ Q) (P ⋀ Q) :=
-  assume h1: dominates σ P' P,
-  show dominates σ (P' ⋀ Q) (P ⋀ Q), from dominates_of (
-    assume h2: σ ⊨ (P' ⋀ Q).instantiated_p,
-
-    have σ ⊨ P'.instantiated_p, from (valid_env.and.elim (valid_env.instantiated_p_and_elim h2)).left,
-    have h3:
-      (σ ⊨ P.instantiated_p) ∧
-      (calls_p_subst σ P ⊆ calls_p_subst σ P') ∧
-      (∀(t': term) (x: var) (Q': prop) (h: callquantifier.mk t' x Q' ∈ quantifiers_p P),
-                            have Q'.size < P.size, from quantifiers_smaller_than_prop.left h,
-      ∃(t: term) (Q: prop), callquantifier.mk t x Q ∈ quantifiers_p P' ∧
-                            (∀v: value, dominates' Q' Q (σ[x↦v]))),
-    from dominates.elim h1 this,
-
-    have h_impl: σ ⊨ (P ⋀ Q).instantiated_p,
-    from valid_env.strengthen_and_with_dominating_instantiations h1 h2,
-
-    have calls_p_subst σ P ⊆ calls_p_subst σ P', from h3.right.left,
-    have h_calls: calls_p_subst σ (P ⋀ Q) ⊆ calls_p_subst σ (P' ⋀ Q), from same_calls_p_and_left this,
-    have h_quantifiers_p:
-      (∀(t': term) (x: var) (Q₁: prop) (h: callquantifier.mk t' x Q₁ ∈ quantifiers_p (P ⋀ Q)),
-                            have Q₁.size < (P ⋀ Q).size, from quantifiers_smaller_than_prop.left h,
-      ∃(t: term) (Q₂: prop), callquantifier.mk t x Q₂ ∈ quantifiers_p (P' ⋀ Q) ∧
-                            (∀v: value, dominates' Q₁ Q₂ (σ[x↦v]))), from (
-
-      assume (t₁: term) (x:var) (Q₁: prop),
-      assume : callquantifier.mk t₁ x Q₁ ∈ quantifiers_p (P ⋀ Q),
-      or.elim (prop.has_quantifier_p.and.inv this) (
-        assume : callquantifier.mk t₁ x Q₁ ∈ quantifiers_p P,
-        have ∃(t₂: term) (Q₂: prop), callquantifier.mk t₂ x Q₂ ∈ quantifiers_p P' ∧
-                            (∀v: value, dominates' Q₁ Q₂ (σ[x↦v])),
-        from h3.right.right t₁ x Q₁ this,
-        let ⟨t₂, Q₂, ⟨call_t₂_Q₂_in_P', Q₂_impl_Q₁⟩⟩ := this in
-        have callquantifier.mk t₂ x Q₂ ∈ quantifiers_p (P' ⋀ Q), from prop.has_quantifier_p.and₁ call_t₂_Q₂_in_P',
-        show ∃(t₂: term) (Q₂: prop), callquantifier.mk t₂ x Q₂ ∈ quantifiers_p (P' ⋀ Q) ∧
-                                    (∀v: value, dominates' Q₁ Q₂ (σ[x↦v])),
-        from exists.intro t₂ (exists.intro Q₂ ⟨this, Q₂_impl_Q₁⟩)
-      ) (
-        assume : callquantifier.mk t₁ x Q₁ ∈ quantifiers_p Q,
-        have h1: callquantifier.mk t₁ x Q₁ ∈ quantifiers_p (P' ⋀ Q), from prop.has_quantifier_p.and₂ this,
-        have h2: ∀v: value, dominates' Q₁ Q₁ (σ[x↦v]), from (
-          assume v: value,
-          show dominates' Q₁ Q₁ (σ[x↦v]), from dominates_self
-        ),
-        show ∃(t₂: term) (Q₂: prop), callquantifier.mk t₂ x Q₂ ∈ quantifiers_p (P' ⋀ Q) ∧
-                                    (∀v: value, dominates' Q₁ Q₂ (σ[x↦v])),
-        from exists.intro t₁ (exists.intro Q₁ ⟨h1, h2⟩)
-      )
-    ),
-    ⟨h_impl, ⟨h_calls, h_quantifiers_p⟩⟩
-  )
-
-lemma dominates_and_symm {P₁ P₂: prop} {σ: env}:
-      dominates σ (P₁ ⋀ P₂) (P₂ ⋀ P₁) :=
-
-  show dominates σ (P₁ ⋀ P₂) (P₂ ⋀ P₁), from dominates_of (
-    assume h0: σ ⊨ (P₁ ⋀ P₂).instantiated_p,
-    have h_impl: σ ⊨ (P₂ ⋀ P₁).instantiated_p, from valid_env.and_symm_with_instantiations h0,
-
-    have h1: calls_p_subst σ (P₁ ⋀ P₂) = (calltrigger.subst σ) '' calls_p (P₁ ⋀ P₂), by unfold calls_p_subst,
-    have calls_p (P₁ ⋀ P₂) = calls_p (P₂ ⋀ P₁), from prop.has_call_p.and.symm,
-    have h2: calls_p_subst σ (P₁ ⋀ P₂) = (calltrigger.subst σ) '' calls_p (P₂ ⋀ P₁),
-    from this ▸ h1,
-    have calls_p_subst σ (P₂ ⋀ P₁) = (calltrigger.subst σ) '' calls_p (P₂ ⋀ P₁), by unfold calls_p_subst,
-    have calls_p_subst σ (P₂ ⋀ P₁) = calls_p_subst σ (P₁ ⋀ P₂), from eq.trans this h2.symm,
-    have h_calls: calls_p_subst σ (P₂ ⋀ P₁) ⊆ calls_p_subst σ (P₁ ⋀ P₂), from set.subset_of_eq this,
-
-    have h_quantifiers_p:
-      (∀(t₁: term) (x: var) (Q₁: prop) (h: callquantifier.mk t₁ x Q₁ ∈ quantifiers_p (P₂ ⋀ P₁)),
-                            have Q₁.size < (P₂ ⋀ P₁).size, from quantifiers_smaller_than_prop.left h,
-      ∃(t₂: term) (Q₂: prop), callquantifier.mk t₂ x Q₂ ∈ quantifiers_p (P₁ ⋀ P₂) ∧
-                            (∀v: value, dominates' Q₁ Q₂ (σ[x↦v]))), from (
-
-      assume (t₁: term) (x:var) (Q₁: prop),
-      assume t₁_Q₁_in_c: callquantifier.mk t₁ x Q₁ ∈ quantifiers_p (P₂ ⋀ P₁),
-      have quantifiers_p (P₂ ⋀ P₁) = quantifiers_p (P₁ ⋀ P₂), from prop.has_quantifier_p.and.symm,
-      have t₁_Q₁_in: callquantifier.mk t₁ x Q₁ ∈ quantifiers_p (P₁ ⋀ P₂), from this ▸ t₁_Q₁_in_c,
-      have (∀v: value, dominates' Q₁ Q₁ (σ[x↦v])), from (
-        assume v: value,
-        dominates_self
-      ),
-
-      show ∃(t₂: term) (Q₂: prop), callquantifier.mk t₂ x Q₂ ∈ quantifiers_p (P₁ ⋀ P₂) ∧
-                                    (∀v: value, dominates' Q₁ Q₂ (σ[x↦v])),
-      from exists.intro t₁ (exists.intro Q₁ ⟨t₁_Q₁_in, this⟩)
-    ),
-
-    ⟨h_impl, ⟨h_calls, h_quantifiers_p⟩⟩
-  )
-
-
-lemma dominates_and_comm {P₁ P₂ P₃: prop} {σ: env}:
-      dominates σ (P₁ ⋀ P₂ ⋀ P₃) ((P₁ ⋀ P₂) ⋀ P₃) :=
-
-  show dominates σ (P₁ ⋀ P₂ ⋀ P₃) ((P₁ ⋀ P₂) ⋀ P₃), from dominates_of (
-    assume h0: σ ⊨ (P₁ ⋀ P₂ ⋀ P₃).instantiated_p,
-    have h_impl: σ ⊨ ((P₁ ⋀ P₂) ⋀ P₃).instantiated_p, from valid_env.and_comm_with_instantiations.mp h0,
-
-    have h1: calls_p_subst σ (P₁ ⋀ P₂ ⋀ P₃) = (calltrigger.subst σ) '' calls_p (P₁ ⋀ P₂ ⋀ P₃), by unfold calls_p_subst,
-    have calls_p (P₁ ⋀ P₂ ⋀ P₃) = calls_p ((P₁ ⋀ P₂) ⋀ P₃), from prop.has_call_p.and.comm,
-    have h2: calls_p_subst σ (P₁ ⋀ P₂ ⋀ P₃) = (calltrigger.subst σ) '' calls_p ((P₁ ⋀ P₂) ⋀ P₃),
-    from this ▸ h1,
-    have calls_p_subst σ ((P₁ ⋀ P₂) ⋀ P₃) = (calltrigger.subst σ) '' calls_p ((P₁ ⋀ P₂) ⋀ P₃), by unfold calls_p_subst,
-    have calls_p_subst σ ((P₁ ⋀ P₂) ⋀ P₃) = calls_p_subst σ (P₁ ⋀ P₂ ⋀ P₃), from eq.trans this h2.symm,
-    have h_calls: calls_p_subst σ ((P₁ ⋀ P₂) ⋀ P₃) ⊆ calls_p_subst σ (P₁ ⋀ P₂ ⋀ P₃), from set.subset_of_eq this,
-
-    have h_quantifiers_p:
-      (∀(t₁: term) (x: var) (Q₁: prop) (h: callquantifier.mk t₁ x Q₁ ∈ quantifiers_p ((P₁ ⋀ P₂) ⋀ P₃)),
-                            have Q₁.size < ((P₁ ⋀ P₂) ⋀ P₃).size, from quantifiers_smaller_than_prop.left h,
-      ∃(t₂: term) (Q₂: prop), callquantifier.mk t₂ x Q₂ ∈ quantifiers_p (P₁ ⋀ P₂ ⋀ P₃) ∧
-                            (∀v: value, dominates' Q₁ Q₂ (σ[x↦v]))), from (
-
-      assume (t₁: term) (x:var) (Q₁: prop),
-      assume t₁_Q₁_in_c: callquantifier.mk t₁ x Q₁ ∈ quantifiers_p ((P₁ ⋀ P₂) ⋀ P₃),
-      have quantifiers_p ((P₁ ⋀ P₂) ⋀ P₃) = quantifiers_p (P₁ ⋀ P₂ ⋀ P₃), from prop.has_quantifier_p.and.comm.symm,
-      have t₁_Q₁_in: callquantifier.mk t₁ x Q₁ ∈ quantifiers_p (P₁ ⋀ P₂ ⋀ P₃), from this ▸ t₁_Q₁_in_c,
-      have (∀v: value, dominates' Q₁ Q₁ (σ[x↦v])), from (
-        assume v: value,
-        dominates_self
-      ),
-
-      show ∃(t₂: term) (Q₂: prop), callquantifier.mk t₂ x Q₂ ∈ quantifiers_p (P₁ ⋀ P₂ ⋀ P₃) ∧
-                                    (∀v: value, dominates' Q₁ Q₂ (σ[x↦v])),
-      from exists.intro t₁ (exists.intro Q₁ ⟨t₁_Q₁_in, this⟩)
-    ),
-
-    ⟨h_impl, ⟨h_calls, h_quantifiers_p⟩⟩
-  )
-
-lemma dominates_and_rcomm {P₁ P₂ P₃: prop} {σ: env}:
-      dominates σ ((P₁ ⋀ P₂) ⋀ P₃) (P₁ ⋀ P₂ ⋀ P₃) :=
-
-  show dominates σ ((P₁ ⋀ P₂) ⋀ P₃) (P₁ ⋀ P₂ ⋀ P₃), from dominates_of (
-    assume h0: σ ⊨ ((P₁ ⋀ P₂) ⋀ P₃).instantiated_p,
-    have h_impl: σ ⊨ (P₁ ⋀ P₂ ⋀ P₃).instantiated_p, from valid_env.and_comm_with_instantiations.mpr h0,
-
-    have h1: calls_p_subst σ (P₁ ⋀ P₂ ⋀ P₃) = (calltrigger.subst σ) '' calls_p (P₁ ⋀ P₂ ⋀ P₃), by unfold calls_p_subst,
-    have calls_p (P₁ ⋀ P₂ ⋀ P₃) = calls_p ((P₁ ⋀ P₂) ⋀ P₃), from prop.has_call_p.and.comm,
-    have h2: calls_p_subst σ (P₁ ⋀ P₂ ⋀ P₃) = (calltrigger.subst σ) '' calls_p ((P₁ ⋀ P₂) ⋀ P₃),
-    from this ▸ h1,
-    have calls_p_subst σ ((P₁ ⋀ P₂) ⋀ P₃) = (calltrigger.subst σ) '' calls_p ((P₁ ⋀ P₂) ⋀ P₃), by unfold calls_p_subst,
-    have calls_p_subst σ ((P₁ ⋀ P₂) ⋀ P₃) = calls_p_subst σ (P₁ ⋀ P₂ ⋀ P₃), from eq.trans this h2.symm,
-    have h_calls: calls_p_subst σ (P₁ ⋀ P₂ ⋀ P₃) ⊆ calls_p_subst σ ((P₁ ⋀ P₂) ⋀ P₃), from set.subset_of_eq this.symm,
-
-    have h_quantifiers_p:
-      (∀(t₁: term) (x: var) (Q₁: prop) (h: callquantifier.mk t₁ x Q₁ ∈ quantifiers_p (P₁ ⋀ P₂ ⋀ P₃)),
-                            have Q₁.size < (P₁ ⋀ P₂ ⋀ P₃).size, from quantifiers_smaller_than_prop.left h,
-      ∃(t₂: term) (Q₂: prop), callquantifier.mk t₂ x Q₂ ∈ quantifiers_p ((P₁ ⋀ P₂) ⋀ P₃) ∧
-                            (∀v: value, dominates' Q₁ Q₂ (σ[x↦v]))), from (
-
-      assume (t₁: term) (x:var) (Q₁: prop),
-      assume t₁_Q₁_in_c: callquantifier.mk t₁ x Q₁ ∈ quantifiers_p (P₁ ⋀ P₂ ⋀ P₃),
-      have quantifiers_p (P₁ ⋀ P₂ ⋀ P₃) = quantifiers_p ((P₁ ⋀ P₂) ⋀ P₃), from prop.has_quantifier_p.and.comm,
-      have t₁_Q₁_in: callquantifier.mk t₁ x Q₁ ∈ quantifiers_p ((P₁ ⋀ P₂) ⋀ P₃), from this ▸ t₁_Q₁_in_c,
-      have (∀v: value, dominates' Q₁ Q₁ (σ[x↦v])), from (
-        assume v: value,
-        dominates_self
-      ),
-
-      show ∃(t₂: term) (Q₂: prop), callquantifier.mk t₂ x Q₂ ∈ quantifiers_p ((P₁ ⋀ P₂) ⋀ P₃) ∧
-                                    (∀v: value, dominates' Q₁ Q₂ (σ[x↦v])),
-      from exists.intro t₁ (exists.intro Q₁ ⟨t₁_Q₁_in, this⟩)
-    ),
-
-    ⟨h_impl, ⟨h_calls, h_quantifiers_p⟩⟩
-  )
-
-lemma dominates.trans: ∀ {P₁ P₂ P₃: prop} {σ: env},
-      dominates σ P₁ P₂ → dominates σ P₂ P₃ → dominates σ P₁ P₃
-| P₁ P₂ P₃ σ :=
-
-  assume h1: dominates σ P₁ P₂,
-  assume h2: dominates σ P₂ P₃,
-  show dominates σ P₁ P₃, from dominates_of (
-    assume : σ ⊨ P₁.instantiated_p,
-
-    have h3:
-      ((σ ⊨ P₂.instantiated_p) ∧
-      (calls_p_subst σ P₂ ⊆ calls_p_subst σ P₁) ∧
-      (∀(t': term) (x: var) (Q': prop) (h: callquantifier.mk t' x Q' ∈ quantifiers_p P₂),
-                            have Q'.size < P₂.size, from quantifiers_smaller_than_prop.left h,
-      ∃(t: term) (Q: prop), callquantifier.mk t x Q ∈ quantifiers_p P₁ ∧
-                            (∀v: value, dominates' Q' Q (σ[x↦v])))),
-    from dominates.elim h1 this,
-
-    have h4:
-      ((σ ⊨ P₃.instantiated_p) ∧
-      (calls_p_subst σ P₃ ⊆ calls_p_subst σ P₂) ∧
-      (∀(t': term) (x: var) (Q': prop) (h: callquantifier.mk t' x Q' ∈ quantifiers_p P₃),
-                            have Q'.size < P₃.size, from quantifiers_smaller_than_prop.left h,
-      ∃(t: term) (Q: prop), callquantifier.mk t x Q ∈ quantifiers_p P₂ ∧
-                            (∀v: value, dominates' Q' Q (σ[x↦v])))),
-    from dominates.elim h2 h3.left,
-
-    have h_impl: (σ ⊨ P₃.instantiated_p), from h4.left,
-
-    have h_calls: calls_p_subst σ P₃ ⊆ calls_p_subst σ P₁,
-    from set.subset.trans h4.right.left h3.right.left,
-
-    have h_quantifiers_p:
-      (∀(t₃: term) (x: var) (Q₃: prop) (h: callquantifier.mk t₃ x Q₃ ∈ quantifiers_p P₃),
-                            have Q₃.size < P₃.size, from quantifiers_smaller_than_prop.left h,
-      ∃(t₁: term) (Q₁: prop), callquantifier.mk t₁ x Q₁ ∈ quantifiers_p P₁ ∧
-                            (∀v: value, dominates' Q₃ Q₁ (σ[x↦v]))), from (
-
-      assume (t₃: term) (x:var) (Q₃: prop),
-      assume h5: callquantifier.mk t₃ x Q₃ ∈ quantifiers_p P₃,
-      have ∃(t: term) (Q₂: prop), callquantifier.mk t x Q₂ ∈ quantifiers_p P₂ ∧
-                            (∀v: value, dominates' Q₃ Q₂ (σ[x↦v])),
-      from h4.right.right t₃ x Q₃ h5,
-      let ⟨t₂, Q₂, ⟨t₂_Q₂_in_P₂, Q₃_dom_Q₂⟩⟩ := this in
-      have ∃(t₁: term) (Q₁: prop), callquantifier.mk t₁ x Q₁ ∈ quantifiers_p P₁ ∧
-                            (∀v: value, dominates' Q₂ Q₁ (σ[x↦v])),
-      from h3.right.right t₂ x Q₂ t₂_Q₂_in_P₂,
-      let ⟨t₁, Q₁, ⟨t₁_Q₁_in_P₁, Q₂_dom_Q₁⟩⟩ := this in
-      have Q₃_dom_Q₁: (∀v: value, dominates' Q₃ Q₁ (σ[x↦v])), from (
-        assume v: value,
-        have h6: dominates (σ[x↦v]) Q₁ Q₂, from Q₂_dom_Q₁ v,
-        have h7: dominates (σ[x↦v]) Q₂ Q₃, from Q₃_dom_Q₂ v,
-        have Q₁.size < P₁.size, from quantifiers_smaller_than_prop.left t₁_Q₁_in_P₁,
-        show dominates (σ[x↦v]) Q₁ Q₃, from dominates.trans h6 h7
-      ),
-
-      show ∃(t₁: term) (Q₁: prop), callquantifier.mk t₁ x Q₁ ∈ quantifiers_p P₁ ∧
-                                  (∀v: value, dominates' Q₃ Q₁ (σ[x↦v])),
-      from exists.intro t₁ (exists.intro Q₁ ⟨t₁_Q₁_in_P₁, Q₃_dom_Q₁⟩)
-    ),
-
-    ⟨h_impl, ⟨h_calls, h_quantifiers_p⟩⟩
-  )
-
-lemma dominates_of_and₁ {P₁ P₂: prop} {σ: env}:
-      dominates σ (P₁ ⋀ P₂) P₁ :=
-
-  show dominates σ (P₁ ⋀ P₂) P₁, from dominates_of (
-
-    assume : σ ⊨ (P₁ ⋀ P₂).instantiated_p,
-    have h_impl: σ ⊨ P₁.instantiated_p,
-    from (valid_env.and.elim (valid_env.instantiated_p_and_elim this)).left,
-
-    have h_calls: calls_p_subst σ P₁ ⊆ calls_p_subst σ (P₁ ⋀ P₂), from (
-      assume c: calltrigger,
-      assume : c ∈ calls_p_subst σ P₁,
-      show c ∈ calls_p_subst σ (P₁ ⋀ P₂), from prop.has_call_p_subst.and₁ this
-    ),
-
-    have h_quantifiers_p:
-      (∀(t₁: term) (x: var) (Q₁: prop) (h: callquantifier.mk t₁ x Q₁ ∈ quantifiers_p P₁),
-                            have Q₁.size < P₁.size, from quantifiers_smaller_than_prop.left h,
-      ∃(t₂: term) (Q₂: prop), callquantifier.mk t₂ x Q₂ ∈ quantifiers_p (P₁ ⋀ P₂) ∧
-                            (∀v: value, dominates' Q₁ Q₂ (σ[x↦v]))), from (
-
-      assume (t₁: term) (x:var) (Q₁: prop),
-      assume t₁_Q₁_in: callquantifier.mk t₁ x Q₁ ∈ quantifiers_p P₁,
-      have t₁_Q₁_in_c: callquantifier.mk t₁ x Q₁ ∈ quantifiers_p (P₁ ⋀ P₂),
-      from prop.has_quantifier_p.and₁ t₁_Q₁_in,
-      have (∀v: value, dominates' Q₁ Q₁ (σ[x↦v])), from (
-        assume v: value,
-        dominates_self
-      ),
-
-      show ∃(t₂: term) (Q₂: prop), callquantifier.mk t₂ x Q₂ ∈ quantifiers_p (P₁ ⋀ P₂) ∧
-                                    (∀v: value, dominates' Q₁ Q₂ (σ[x↦v])),
-      from exists.intro t₁ (exists.intro Q₁ ⟨t₁_Q₁_in_c, this⟩)
-    ),
-    ⟨h_impl, ⟨h_calls, h_quantifiers_p⟩⟩
-  )
-
-
-lemma dominates_of_and₂ {P₁ P₂: prop} {σ: env}:
-      dominates σ (P₁ ⋀ P₂) P₂ :=
-  have h1: dominates σ (P₁ ⋀ P₂) (P₂ ⋀ P₁), from dominates_and_symm,
-  have h2: dominates σ (P₂ ⋀ P₁) P₂, from dominates_of_and₁,
-  show dominates σ (P₁ ⋀ P₂) P₂, from dominates.trans h1 h2
-
-lemma dominates_not_not {P: prop} {σ: env}:
-      dominates σ P.not.not P :=
-  show dominates σ P.not.not P, from dominates_of (
-    assume h1: σ ⊨ P.not.not.instantiated_p,
-    have P.not.not.instantiated_p = P.not.instantiated_n.not, from not_dist_instantiated_p,
-    have h2: σ ⊨ P.not.instantiated_n.not, from this ▸ h1,
-    have P.not.instantiated_n = P.instantiated_p.not, from not_dist_instantiated_n,
-    have σ ⊨ P.instantiated_p.not.not, from this ▸ h2,
-    have h_impl: σ ⊨ P.instantiated_p, from valid_env.neg_neg.mp this,
-    have h_calls: calls_p_subst σ P ⊆ calls_p_subst σ P.not.not, from (
-      assume c: calltrigger,
-      assume : c ∈ calls_p_subst σ P,
-      have c ∈ calls_n_subst σ P.not, from prop.has_call_p_subst.not this,
-      show c ∈ calls_p_subst σ P.not.not, from prop.has_call_n_subst.not this
-    ),
-    have h_quantifiers_p:
-      (∀(t': term) (x: var) (Q₁: prop) (h: callquantifier.mk t' x Q₁ ∈ quantifiers_p P),
-                            have Q₁.size < P.size, from quantifiers_smaller_than_prop.left h,
-      ∃(t: term) (Q₂: prop), callquantifier.mk t x Q₂ ∈ quantifiers_p P.not.not ∧
-                            (∀v: value, dominates' Q₁ Q₂ (σ[x↦v]))), from (
-      assume (t₁: term) (x:var) (Q₁: prop),
-      assume h: callquantifier.mk t₁ x Q₁ ∈ quantifiers_p P,
-      have callquantifier.mk t₁ x Q₁ ∈ quantifiers_n P.not, from prop.has_quantifier_n.not h,
-      have h2: callquantifier.mk t₁ x Q₁ ∈ quantifiers_p P.not.not, from prop.has_quantifier_p.not this,
-      have Q₁.size < P.size, from quantifiers_smaller_than_prop.left h,
-      have (∀v: value, dominates' Q₁ Q₁ (σ[x↦v])), from (
-        assume v: value,
-        dominates_self
-      ),
-      exists.intro t₁ (exists.intro Q₁ ⟨h2, this⟩)
-    ),
-    ⟨h_impl, ⟨h_calls, h_quantifiers_p⟩⟩
-  )
-
-lemma dominates_of_not_not {P: prop} {σ: env}:
-      dominates σ P P.not.not :=
-  show dominates σ P P.not.not, from dominates_of (
-    assume : σ ⊨ P.instantiated_p,
-    have h1: σ ⊨ P.instantiated_p.not.not, from valid_env.neg_neg.mpr this,
-    have P.not.instantiated_n = P.instantiated_p.not, from not_dist_instantiated_n,
-    have h2: σ ⊨ P.not.instantiated_n.not, from this.symm ▸ h1,
-    have P.not.not.instantiated_p = P.not.instantiated_n.not, from not_dist_instantiated_p,
-    have h_impl: σ ⊨ P.not.not.instantiated_p, from this.symm ▸ h2,
-    have h_calls: calls_p_subst σ P.not.not ⊆ calls_p_subst σ P, from (
-      assume c: calltrigger,
-      assume : c ∈ calls_p_subst σ P.not.not,
-      have c ∈ calls_n_subst σ P.not, from prop.has_call_p_subst.not.inv this,
-      show c ∈ calls_p_subst σ P, from prop.has_call_n_subst.not.inv this
-    ),
-    have h_quantifiers_p:
-      (∀(t': term) (x: var) (Q₁: prop) (h: callquantifier.mk t' x Q₁ ∈ quantifiers_p P.not.not),
-                            have Q₁.size < P.not.not.size, from quantifiers_smaller_than_prop.left h,
-      ∃(t: term) (Q₂: prop), callquantifier.mk t x Q₂ ∈ quantifiers_p P ∧
-                            (∀v: value, dominates' Q₁ Q₂ (σ[x↦v]))), from (
-      assume (t₁: term) (x:var) (Q₁: prop),
-      assume h: callquantifier.mk t₁ x Q₁ ∈ quantifiers_p P.not.not,
-      have callquantifier.mk t₁ x Q₁ ∈ quantifiers_n P.not, from prop.has_quantifier_p.not.inv h,
-      have h2: callquantifier.mk t₁ x Q₁ ∈ quantifiers_p P, from prop.has_quantifier_n.not.inv this,
-      have Q₁.size < P.size, from quantifiers_smaller_than_prop.left h2,
-      have (∀v: value, dominates' Q₁ Q₁ (σ[x↦v])), from (
-        assume v: value,
-        dominates_self
-      ),
-      exists.intro t₁ (exists.intro Q₁ ⟨h2, this⟩)
-    ),
-    ⟨h_impl, ⟨h_calls, h_quantifiers_p⟩⟩
-  )
-
 lemma dominates_true (σ: env) (P: prop):
       dominates σ P value.true :=
-  show dominates σ P value.true, from dominates_of (
-    assume : σ ⊨ P.instantiated_p,
-    have h1: σ ⊨ value.true, from valid_env.true,
-    have (prop.term value.true).erased_n = vc.term value.true, by unfold prop.erased_n,
-    have h2: σ ⊨ (prop.term value.true).erased_n, from this ▸ h1,
-    have calls_p (prop.term value.true) = ∅, from set.eq_empty_of_forall_not_mem (
-      assume c: calltrigger,
-      assume : c ∈ calls_p (prop.term value.true),
-      show «false», from prop.has_call_p.term.inv this
-    ),
-    have (prop.term value.true).instantiated_p = (prop.term value.true).erased_p,
-    from instantiated_p_eq_erased_p_without_calls this,
-    have h_impl: σ ⊨ (prop.term value.true).instantiated_p, from this.symm ▸ h2,
-    have h_calls: calls_p_subst σ value.true ⊆ calls_p_subst σ P, from (
-      assume c: calltrigger,
-      assume : c ∈ calls_p_subst σ value.true,
-      show c ∈ calls_p_subst σ P, from absurd this prop.has_call_p_subst.term.inv
-    ),
-    have h_quantifiers_p:
-      (∀(t': term) (x: var) (Q₁: prop) (h: callquantifier.mk t' x Q₁ ∈ quantifiers_p value.true),
-      ∃(t: term) (Q₂: prop), callquantifier.mk t x Q₂ ∈ quantifiers_p P ∧
-                            (∀v: value, dominates' Q₁ Q₂ (σ[x↦v]))), from (
-      assume (t₁: term) (x:var) (Q₁: prop),
-      assume : callquantifier.mk t₁ x Q₁ ∈ quantifiers_p value.true,
-      show ∃(t: term) (Q₂: prop), callquantifier.mk t x Q₂ ∈ quantifiers_p P ∧
-                                  (∀v: value, dominates' Q₁ Q₂ (σ[x↦v])),
-      from absurd this prop.has_quantifier_p.term.inv
-    ),
-    have h5: closed_subst σ (prop.term value.true), from (
-      assume x: var,
-      assume : free_in_prop x value.true,
-      have free_in_term x value.true, from free_in_prop.term.inv this,
-      show x ∈ σ.dom, from absurd this free_in_term.value.inv
-    ),
-     ⟨h_impl, ⟨h_calls, h_quantifiers_p⟩⟩
-  )
 
-lemma dominates_shuffle {P Q R S: prop} {σ: env}:
-      dominates σ (P ⋀ Q ⋀ R ⋀ S) ((P ⋀ Q ⋀ R) ⋀ S):=
-  have h1: dominates σ (P ⋀ Q ⋀ R ⋀ S) ((Q ⋀ R ⋀ S) ⋀ P), from dominates_and_symm,
-  have h2: dominates σ ((Q ⋀ R ⋀ S) ⋀ P) (((Q ⋀ R) ⋀ S) ⋀ P), from dominates_and_left dominates_and_comm,
-  have h3: dominates σ  (((Q ⋀ R) ⋀ S) ⋀ P) ((Q ⋀ R) ⋀ S ⋀ P), from dominates_and_rcomm,
-  have h4: dominates σ ((Q ⋀ R) ⋀ S ⋀ P) ((S ⋀ P) ⋀ Q ⋀ R), from dominates_and_symm,
-  have h5: dominates σ ((S ⋀ P) ⋀ Q ⋀ R) (S ⋀ P ⋀ Q ⋀ R), from dominates_and_rcomm,
-  have h6: dominates σ (S ⋀ P ⋀ Q ⋀ R) ((P ⋀ Q ⋀ R) ⋀ S), from dominates_and_symm,
-  show dominates σ  (P ⋀ Q ⋀ R ⋀ S) ((P ⋀ Q ⋀ R) ⋀ S),
-  from dominates.trans h1 (dominates.trans h2 (dominates.trans h3 (dominates.trans h4 (dominates.trans h5 h6))))
+  have h1: σ ⊨ value.true, from valid_env.true,
+  have (prop.term value.true).erased_n = vc.term value.true, by unfold prop.erased_n,
+  have h2: σ ⊨ (prop.term value.true).erased_n, from this ▸ h1,
+  have calls_p (prop.term value.true) = ∅, from set.eq_empty_of_forall_not_mem (
+    assume c: calltrigger,
+    assume : c ∈ calls_p (prop.term value.true),
+    show «false», from prop.has_call_p.term.inv this
+  ),
+  have (prop.term value.true).instantiated_p = (prop.term value.true).erased_p,
+  from instantiated_p_eq_erased_p_without_calls this,
+  have h_impl: (σ ⊨ P.instantiated_p) → σ ⊨ (prop.term value.true).instantiated_p, from (λ_, this.symm ▸ h2),
+  have h_calls: calls_p_subst σ value.true ⊆ calls_p_subst σ P, from (
+    assume c: calltrigger,
+    assume : c ∈ calls_p_subst σ value.true,
+    show c ∈ calls_p_subst σ P, from absurd this prop.has_call_p_subst.term.inv
+  ),
+  have h_quantifiers: quantifiers_p value.true = ∅, from set.eq_empty_of_forall_not_mem (
+    assume q: callquantifier,
+    assume : q ∈ quantifiers_p value.true,
+    show «false», from prop.has_quantifier_p.term.inv this
+  ),
+  show dominates σ P value.true, from dominates.no_quantifiers h_impl h_calls h_quantifiers
 
 lemma exp.vcgen.inj {P: prop} {Q: propctx} {e: exp}: (P ⊢ e : Q) → ∀Q', (P ⊢ e : Q') → (Q = Q') :=
   assume h1: P ⊢ e : Q,
@@ -755,117 +364,26 @@ lemma env_equiv_of_translation_valid {σ: env} {P: prop}:
     }
   end
 
-
 lemma env_dominates_rest {P: prop} {σ: env} {x: var} {v: value}:
       (⊢ (σ[x↦v]) : P) → (∃Q, (⊢ σ : Q) ∧ ∀σ', dominates σ' P Q) :=
   assume σ_verified: ⊢ (σ[x↦v]) : P,
   begin
     cases σ_verified,
     case env.vcgen.tru Q _ σ_verified ih { from
-      have ∀σ', dominates σ' (prop.and Q (x ≡ value.true)) Q, from (
-        assume σ': env,
-        show dominates σ' (Q ⋀ x ≡ value.true) Q, from dominates_of (
-          assume h2: σ' ⊨ (Q ⋀ (x ≡ value.true)).instantiated_p,
-          have no_instantiations (x ≡ value.true), from no_instantiations.term,
-          have (Q ⋀ (x ≡ value.true)).instantiated_p = (Q.instantiated_p ⋀ prop.erased_p (x ≡ value.true)),
-          from and_dist_of_no_instantiations_p this,
-          have σ' ⊨ (Q.instantiated_p ⋀ prop.erased_p (x ≡ value.true)), from this ▸ h2,
-          have h_impl: σ' ⊨ Q.instantiated_p, from (valid_env.and.elim this).left,
-          have h_calls: calls_p_subst σ' Q ⊆ calls_p_subst σ' (Q ⋀ x ≡ value.true), from (
-            assume c: calltrigger,
-            assume : c ∈ calls_p_subst σ' Q,
-            show c ∈ calls_p_subst σ' (Q ⋀ x ≡ value.true), from prop.has_call_p_subst.and₁ this
-          ),
-          have h_quantifiers_p:
-            (∀(t': term) (y: var) (Q₁: prop) (h: callquantifier.mk t' y Q₁ ∈ quantifiers_p Q),
-                                  have Q₁.size < Q.size, from quantifiers_smaller_than_prop.left h,
-            ∃(t: term) (Q₂: prop), callquantifier.mk t y Q₂ ∈ quantifiers_p (Q ⋀ x ≡ value.true) ∧
-                                  (∀v: value, dominates' Q₁ Q₂ (σ'[y↦v]))), from (
-            assume (t₁: term) (y:var) (Q₁: prop),
-            assume h: callquantifier.mk t₁ y Q₁ ∈ quantifiers_p Q,
-            have h2: callquantifier.mk t₁ y Q₁ ∈ quantifiers_p (Q ⋀ x ≡ value.true), from prop.has_quantifier_p.and₁ h,
-            have Q₁.size < (Q ⋀ x ≡ value.true).size, from quantifiers_smaller_than_prop.left h2,
-            have (∀v: value, dominates' Q₁ Q₁ (σ'[y↦v])), from (
-              assume v: value,
-              dominates_self
-            ),
-            exists.intro t₁ (exists.intro Q₁ ⟨h2, this⟩)
-          ),
-          ⟨h_impl, ⟨h_calls, h_quantifiers_p⟩⟩
-        )
-      ),
+      have ∀σ', dominates σ' (prop.and Q (x ≡ value.true)) Q,
+      from λσ', dominates.of_and_left,
       show ∃(Q_1 : prop), (⊢ σ : Q_1) ∧ ∀σ', dominates σ' (prop.and Q (x ≡ value.true)) Q_1,
       from exists.intro Q ⟨σ_verified, this⟩
     },
     case env.vcgen.fls Q _ σ_verified { from
-      have ∀σ', dominates σ' (prop.and Q (x ≡ value.false)) Q, from (
-        assume σ': env,
-        show dominates σ' (Q ⋀ x ≡ value.false) Q, from dominates_of (
-          assume h2: σ' ⊨ (Q ⋀ (x ≡ value.false)).instantiated_p,
-          have no_instantiations (x ≡ value.false), from no_instantiations.term,
-          have (Q ⋀ (x ≡ value.false)).instantiated_p = (Q.instantiated_p ⋀ prop.erased_p (x ≡ value.false)),
-          from and_dist_of_no_instantiations_p this,
-          have σ' ⊨ (Q.instantiated_p ⋀ prop.erased_p (x ≡ value.false)), from this ▸ h2,
-          have h_impl: σ' ⊨ Q.instantiated_p, from (valid_env.and.elim this).left,
-          have h_calls: calls_p_subst σ' Q ⊆ calls_p_subst σ' (Q ⋀ x ≡ value.false), from (
-            assume c: calltrigger,
-            assume : c ∈ calls_p_subst σ' Q,
-            show c ∈ calls_p_subst σ' (Q ⋀ x ≡ value.false), from prop.has_call_p_subst.and₁ this
-          ),
-          have h_quantifiers_p:
-            (∀(t': term) (y: var) (Q₁: prop) (h: callquantifier.mk t' y Q₁ ∈ quantifiers_p Q),
-                                  have Q₁.size < Q.size, from quantifiers_smaller_than_prop.left h,
-            ∃(t: term) (Q₂: prop), callquantifier.mk t y Q₂ ∈ quantifiers_p (Q ⋀ x ≡ value.false) ∧
-                                  (∀v: value, dominates' Q₁ Q₂ (σ'[y↦v]))), from (
-            assume (t₁: term) (y:var) (Q₁: prop),
-            assume h: callquantifier.mk t₁ y Q₁ ∈ quantifiers_p Q,
-            have h2: callquantifier.mk t₁ y Q₁ ∈ quantifiers_p (Q ⋀ x ≡ value.false), from prop.has_quantifier_p.and₁ h,
-            have Q₁.size < (Q ⋀ x ≡ value.false).size, from quantifiers_smaller_than_prop.left h2,
-            have (∀v: value, dominates' Q₁ Q₁ (σ'[y↦v])), from (
-              assume v: value,
-              dominates_self
-            ),
-            exists.intro t₁ (exists.intro Q₁ ⟨h2, this⟩)
-          ),
-          ⟨h_impl, ⟨h_calls, h_quantifiers_p⟩⟩
-        )
-      ),
+      have ∀σ', dominates σ' (prop.and Q (x ≡ value.false)) Q,
+      from λσ', dominates.of_and_left,
       show ∃(Q_1 : prop), (⊢ σ : Q_1) ∧ ∀σ', dominates σ' (prop.and Q (x ≡ value.false)) Q_1,
       from exists.intro Q ⟨σ_verified, this⟩
     },
     case env.vcgen.num n Q _ σ_verified { from
-      have ∀σ', dominates σ' (prop.and Q (x ≡ value.num n)) Q, from (
-        assume σ': env,
-        show dominates σ' (Q ⋀ x ≡ value.num n) Q, from dominates_of (
-          assume h2: σ' ⊨ (Q ⋀ (x ≡ value.num n)).instantiated_p,
-          have no_instantiations (x ≡ value.num n), from no_instantiations.term,
-          have (Q ⋀ (x ≡ value.num n)).instantiated_p = (Q.instantiated_p ⋀ prop.erased_p (x ≡ value.num n)),
-          from and_dist_of_no_instantiations_p this,
-          have σ' ⊨ (Q.instantiated_p ⋀ prop.erased_p (x ≡ value.num n)), from this ▸ h2,
-          have h_impl: σ' ⊨ Q.instantiated_p, from (valid_env.and.elim this).left,
-          have h_calls: calls_p_subst σ' Q ⊆ calls_p_subst σ' (Q ⋀ x ≡ value.num n), from (
-            assume c: calltrigger,
-            assume : c ∈ calls_p_subst σ' Q,
-            show c ∈ calls_p_subst σ' (Q ⋀ x ≡ value.num n), from prop.has_call_p_subst.and₁ this
-          ),
-          have h_quantifiers_p:
-            (∀(t': term) (y: var) (Q₁: prop) (h: callquantifier.mk t' y Q₁ ∈ quantifiers_p Q),
-                                  have Q₁.size < Q.size, from quantifiers_smaller_than_prop.left h,
-            ∃(t: term) (Q₂: prop), callquantifier.mk t y Q₂ ∈ quantifiers_p (Q ⋀ x ≡ value.num n) ∧
-                                  (∀v: value, dominates' Q₁ Q₂ (σ'[y↦v]))), from (
-            assume (t₁: term) (y:var) (Q₁: prop),
-            assume h: callquantifier.mk t₁ y Q₁ ∈ quantifiers_p Q,
-            have h2: callquantifier.mk t₁ y Q₁ ∈ quantifiers_p (Q ⋀ x ≡ value.num n), from prop.has_quantifier_p.and₁ h,
-            have Q₁.size < (Q ⋀ x ≡ value.num n).size, from quantifiers_smaller_than_prop.left h2,
-            have (∀v: value, dominates' Q₁ Q₁ (σ'[y↦v])), from (
-              assume v: value,
-              dominates_self
-            ),
-            exists.intro t₁ (exists.intro Q₁ ⟨h2, this⟩)
-          ),
-          ⟨h_impl, ⟨h_calls, h_quantifiers_p⟩⟩
-        )
-      ),
+      have ∀σ', dominates σ' (prop.and Q (x ≡ value.num n)) Q,
+      from λσ', dominates.of_and_left,
       show ∃(Q_1 : prop), (⊢ σ : Q_1) ∧ ∀σ', dominates σ' (prop.and Q (x ≡ value.num n)) Q_1,
       from exists.intro Q ⟨σ_verified, this⟩
     },
@@ -873,41 +391,19 @@ lemma env_dominates_rest {P: prop} {σ: env} {x: var} {v: value}:
          fx_not_in_σ₂ f_neq_fx σ₁_verified σ₂_verified fx_in_R fv_R fv_S e_verified func_vc { from
       let funcp := prop.subst_env (σ₂[f↦value.func f fx R S e H σ₂])
                                   (prop.func f fx R (Q₃ (term.app f fx) ⋀ S)) in
-      have ∀σ', dominates σ' (Q ⋀ x ≡ value.func f fx R S e H σ₂ ⋀ funcp) Q, from (
-        assume σ': env,
-        show dominates σ' (Q ⋀ x ≡ value.func f fx R S e H σ₂ ⋀ funcp) Q, from dominates_of (
-          assume : σ' ⊨ (Q ⋀ x ≡ value.func f fx R S e H σ₂ ⋀ funcp).instantiated_p,
-          have h2: σ' ⊨ Q.instantiated_p ⋀ (↑(x ≡ value.func f fx R S e H σ₂) ⋀ funcp).instantiated_p,
-          from valid_env.instantiated_p_and_elim this,
-          have h_impl: σ' ⊨ Q.instantiated_p, from (valid_env.and.elim h2).left,
-          have h_calls: calls_p_subst σ' Q ⊆ calls_p_subst σ' (Q ⋀ x ≡ value.func f fx R S e H σ₂ ⋀ funcp), from (
-            assume c: calltrigger,
-            assume : c ∈ calls_p_subst σ' Q,
-            show c ∈ calls_p_subst σ' (Q ⋀ x ≡ value.func f fx R S e H σ₂ ⋀ funcp), from prop.has_call_p_subst.and₁ this
-          ),
-          have h_quantifiers_p:
-            (∀(t': term) (y: var) (Q₁: prop) (h: callquantifier.mk t' y Q₁ ∈ quantifiers_p Q),
-                                  have Q₁.size < Q.size, from quantifiers_smaller_than_prop.left h,
-            ∃(t: term) (Q₂: prop), callquantifier.mk t y Q₂ ∈ quantifiers_p (Q ⋀ x ≡ value.func f fx R S e H σ₂ ⋀ funcp) ∧
-                                  (∀v: value, dominates' Q₁ Q₂ (σ'[y↦v]))), from (
-            assume (t₁: term) (y:var) (Q₁: prop),
-            assume h: callquantifier.mk t₁ y Q₁ ∈ quantifiers_p Q,
-            have h2: callquantifier.mk t₁ y Q₁ ∈ quantifiers_p (Q ⋀ x ≡ value.func f fx R S e H σ₂ ⋀ funcp),
-            from prop.has_quantifier_p.and₁ h,
-            have Q₁.size < (Q ⋀ x ≡ value.func f fx R S e H σ₂ ⋀ funcp).size, from quantifiers_smaller_than_prop.left h2,
-            have (∀v: value, dominates' Q₁ Q₁ (σ'[y↦v])), from (
-              assume v: value,
-              dominates_self
-            ),
-            exists.intro t₁ (exists.intro Q₁ ⟨h2, this⟩)
-          ),
-          ⟨h_impl, ⟨h_calls, h_quantifiers_p⟩⟩
-        )
-      ),
+      have ∀σ', dominates σ' (Q ⋀ x ≡ value.func f fx R S e H σ₂ ⋀ funcp) Q,
+      from λσ', dominates.of_and_left,
       show ∃Q_1, (⊢ σ : Q_1) ∧ ∀σ', dominates σ' (prop.and Q ((x ≡ (value.func f fx R S e H σ₂)) ⋀ funcp)) Q_1,
       from exists.intro Q ⟨σ₁_verified, this⟩
     }
   end
+
+lemma strengthen_and_with_dominating_instantiations {σ: env} {P P' Q: prop}:
+  dominates σ P P' → (σ ⊨ (P ⋀ Q).instantiated_p) → σ ⊨ (P' ⋀ Q).instantiated_p :=
+  assume h1: dominates σ P P',
+  assume h2: (σ ⊨ (P ⋀ Q).instantiated_p),
+  have dominates σ (P ⋀ Q) (P' ⋀ Q), from dominates.same_right (λ_, h1),
+  dominates.elim this h2
 
 lemma strengthen_impl_with_dominating_instantiations {σ: env} {P P' Q: prop}:
   dominates σ P' P → FV P' ⊆ FV P → (σ ⊨ (prop.implies P Q).instantiated_n) → (σ ⊨ (prop.implies P' Q).instantiated_n) :=
@@ -928,7 +424,7 @@ lemma strengthen_impl_with_dominating_instantiations {σ: env} {P P' Q: prop}:
       show y ∈ FV P.not, from free_in_prop.not this
     ),
     have FV (P'.not ⋁ Q).instantiated_n ⊆ FV (P.not ⋁ Q).instantiated_n,
-    from free_in_prop.strengthen_or_with_dominating_instantiations this,
+    from free_in_prop.strengthen_or_with_instantiations this,
     have x ∈ FV (P.not ⋁ Q).instantiated_n, from set.mem_of_subset_of_mem this h13,
     show x ∈ σ.dom,
     from set.mem_of_subset_of_mem (valid_env.closed h0) this
@@ -945,14 +441,14 @@ lemma strengthen_impl_with_dominating_instantiations {σ: env} {P P' Q: prop}:
     have h43: P'.not.instantiated_n = P'.instantiated_p.not, from not_dist_instantiated_n,
     have σ ⊨ P'.instantiated_p.not.not, from h43 ▸ h42 ▸ h41,
     have σ ⊨ P'.instantiated_p, from valid_env.neg_neg.mp this,
-    have dominates σ P'.not.not P', from dominates_not_not,
+    have dominates σ P'.not.not P', from dominates.not_not,
     have h5: σ ⊨ (P' ⋀ Q.not).instantiated_p,
-    from valid_env.strengthen_and_with_dominating_instantiations this h4,
+    from strengthen_and_with_dominating_instantiations this h4,
     have h6: σ ⊨ (P ⋀ Q.not).instantiated_p,
-    from valid_env.strengthen_and_with_dominating_instantiations P'_dominates_P h5,
-    have dominates σ P P.not.not, from dominates_of_not_not,
+    from strengthen_and_with_dominating_instantiations P'_dominates_P h5,
+    have dominates σ P P.not.not, from dominates.of_not_not,
     have σ ⊨ (P.not.not ⋀ Q.not).instantiated_p,
-    from valid_env.strengthen_and_with_dominating_instantiations this h6,
+    from strengthen_and_with_dominating_instantiations this h6,
     show σ ⊨ (P.not ⋁ Q).not.instantiated_p, from valid_env.or_not_dist_with_instantiations.mpr this
   ),
   have ¬ σ ⊨ (P'.not ⋁ Q).not.instantiated_p, from mt h3 h2,
@@ -966,7 +462,7 @@ lemma strengthen_vc {P P' Q S: prop} {σ: env}:
   (σ ⊨ (prop.implies (P ⋀ Q) S).instantiated_n) → σ ⊨ (prop.implies (P' ⋀ Q) S).instantiated_n :=
   assume : dominates σ P' P,
   assume fv_P'_P: FV P' ⊆ FV P,
-  have h1: dominates σ (P' ⋀ Q) (P ⋀ Q), from dominates_and_left this,
+  have h1: dominates σ (P' ⋀ Q) (P ⋀ Q), from dominates.same_right (λ_, this),
   have h2: FV (P' ⋀ Q) ⊆ FV (P ⋀ Q), from (
     assume x: var,
     assume : x ∈ FV (P' ⋀ Q),
@@ -994,7 +490,7 @@ lemma strengthen_exp {P: prop} {Q: propctx} {e: exp}:
       have h1: FV (P' ⋀ x ≡ value.true) = FV (P ⋀ x ≡ value.true),
       from same_free_and_left free_P'_P,
       have h2: (∀σ, dominates σ (P' ⋀ x ≡ value.true) (P ⋀ x ≡ value.true)),
-      from λσ, dominates_and_left (P'_dominates_P σ),
+      from λσ, dominates.same_right (λ_, P'_dominates_P σ),
       have e'_verified': P' ⋀ x ≡ value.true ⊢ e': Q, from ih (P' ⋀ x ≡ value.true) h1 h2,
       have x_not_free_in_P': x ∉ FV P', from free_P'_P.symm ▸ x_not_free_in_P,
       show P' ⊢ lett x = true in e' : propctx.exis x (x ≡ value.true ⋀ Q),
@@ -1008,7 +504,7 @@ lemma strengthen_exp {P: prop} {Q: propctx} {e: exp}:
       have h1: FV (P' ⋀ (x ≡ value.false)) = FV (P ⋀ x ≡ value.false),
       from same_free_and_left free_P'_P,
       have h2: (∀σ, dominates σ (P' ⋀ x ≡ value.false) (P ⋀ x ≡ value.false)),
-      from λσ, dominates_and_left (P'_dominates_P σ),
+      from λσ, dominates.same_right (λ_, P'_dominates_P σ),
       have e'_verified': P' ⋀ x ≡ value.false ⊢ e': Q, from ih (P' ⋀ x ≡ value.false) h1 h2,
       have x_not_free_in_P': x ∉ FV P', from free_P'_P.symm ▸ x_not_free_in_P,
       show P' ⊢ letf x = false in e' : propctx.exis x ((x ≡ value.false) ⋀ Q),
@@ -1022,7 +518,7 @@ lemma strengthen_exp {P: prop} {Q: propctx} {e: exp}:
       have h1: FV (P' ⋀ x ≡ value.num n) = FV (P ⋀ x ≡ value.num n),
       from same_free_and_left free_P'_P,
       have h2: (∀σ, dominates σ (P' ⋀ x ≡ value.num n) (P ⋀ x ≡ value.num n)),
-      from λσ, dominates_and_left (P'_dominates_P σ),
+      from λσ, dominates.same_right (λ_, P'_dominates_P σ),
       have e'_verified': P' ⋀ (x ≡ value.num n) ⊢ e': Q, from ih (P' ⋀ (x ≡ value.num n)) h1 h2,
       have x_not_free_in_P': x ∉ FV P', from free_P'_P.symm ▸ x_not_free_in_P,
       show P' ⊢ letn x = n in e' : propctx.exis x ((x ≡ value.num n) ⋀ Q),
@@ -1042,7 +538,7 @@ lemma strengthen_exp {P: prop} {Q: propctx} {e: exp}:
       have h1: FV (P' ⋀ ((spec.func f x R S) ⋀ R)) = FV (P ⋀ ((spec.func f x R S) ⋀ R)),
       from same_free_and_left free_P'_P,
       have h2: (∀σ, dominates σ (P' ⋀ (spec.func f x R S) ⋀ R) (P ⋀ (spec.func f x R S) ⋀ R)),
-      from λσ, dominates_and_left (P'_dominates_P σ),
+      from λσ, dominates.same_right (λ_, P'_dominates_P σ),
       have e₁_verified': P' ⋀ (spec.func f x R S) ⋀ R ⊢ e₁ : Q₁,
       from ih₁ (P' ⋀ (spec.func f x R S) ⋀ R) h1 h2,
 
@@ -1052,7 +548,7 @@ lemma strengthen_exp {P: prop} {Q: propctx} {e: exp}:
 
       have h5: (∀σ, dominates σ (P' ⋀ (prop.func f x R (Q₁ (term.app ↑f ↑x) ⋀ ↑S)))
                       (P ⋀ (prop.func f x R (Q₁ (term.app ↑f ↑x) ⋀ ↑S)))),
-      from (λσ, dominates_and_left (P'_dominates_P σ)),
+      from (λσ, dominates.same_right (λ_, P'_dominates_P σ)),
 
       have e₂_verified': P' ⋀ (prop.func f x R (Q₁ (term.app ↑f ↑x) ⋀ ↑S)) ⊢ e₂ : Q₂,
       from ih₂ (P' ⋀ (prop.func f x R (Q₁ (term.app ↑f ↑x) ⋀ ↑S))) h3 h5,
@@ -1076,7 +572,7 @@ lemma strengthen_exp {P: prop} {Q: propctx} {e: exp}:
       have h1: FV (P' ⋀ y ≡ term.unop op x) = FV (P ⋀ y ≡ term.unop op x),
       from same_free_and_left free_P'_P,
       have h2: (∀σ, dominates σ (P' ⋀ y ≡ term.unop op x) (P ⋀ y ≡ term.unop op x)),
-      from (λσ, dominates_and_left (P'_dominates_P σ)),
+      from (λσ, dominates.same_right (λ_, P'_dominates_P σ)),
       have e'_verified': P' ⋀ y ≡ term.unop op x ⊢ e' : Q',
       from ih (P' ⋀ y ≡ term.unop op x) h1 h2,
 
@@ -1099,7 +595,7 @@ lemma strengthen_exp {P: prop} {Q: propctx} {e: exp}:
       have h1: FV (P' ⋀ z ≡ term.binop op x y) = FV (P ⋀ z ≡ term.binop op x y),
       from same_free_and_left free_P'_P,
       have h2: (∀σ, dominates σ (P' ⋀ z ≡ term.binop op x y) (P ⋀ z ≡ term.binop op x y)),
-      from (λσ, dominates_and_left (P'_dominates_P σ)),
+      from (λσ, dominates.same_right (λ_, P'_dominates_P σ)),
       have e'_verified': P' ⋀ z ≡ term.binop op x y ⊢ e' : Q',
       from ih (P' ⋀ z ≡ term.binop op x y) h1 h2,
 
@@ -1125,7 +621,7 @@ lemma strengthen_exp {P: prop} {Q: propctx} {e: exp}:
 
       have h2: (∀σ, dominates σ (P' ⋀ prop.call f x ⋀ prop.post f x ⋀ y ≡ term.app f x)
                                 (P ⋀ prop.call f x ⋀ prop.post f x ⋀ y ≡ term.app f x)),
-      from (λσ, dominates_and_left (P'_dominates_P σ)),
+      from (λσ, dominates.same_right (λ_, P'_dominates_P σ)),
 
       have e'_verified': P' ⋀ prop.call f x ⋀ prop.post f x ⋀ y ≡ term.app f x ⊢ e' : Q',
       from ih (P' ⋀ prop.call f x ⋀ prop.post f x ⋀ y ≡ term.app f x) h1 h2,
@@ -1145,12 +641,12 @@ lemma strengthen_exp {P: prop} {Q: propctx} {e: exp}:
       have x_free_in_P': x ∈ FV P', from free_P'_P.symm ▸ x_free_in_P,
 
       have h1: FV (P' ⋀ x) = FV (P ⋀ x), from same_free_and_left free_P'_P,
-      have h2: (∀σ, dominates σ (P' ⋀ x) (P ⋀ x)), from (λσ, dominates_and_left (P'_dominates_P σ)),
+      have h2: (∀σ, dominates σ (P' ⋀ x) (P ⋀ x)), from (λσ, dominates.same_right (λ_, P'_dominates_P σ)),
       have e₁_verified': P' ⋀ x ⊢ e₁ : Q₁, from ih₁ (P' ⋀ x) h1 h2,
 
       have h1: FV (P' ⋀ term.unop unop.not x) = FV (P ⋀ term.unop unop.not x), from same_free_and_left free_P'_P,
       have h2: (∀σ, dominates σ (P' ⋀ term.unop unop.not x) (P ⋀ term.unop unop.not x)),
-      from (λσ, dominates_and_left (P'_dominates_P σ)),
+      from (λσ, dominates.same_right (λ_, P'_dominates_P σ)),
       have e₂_verified': P' ⋀ term.unop unop.not x ⊢ e₂ : Q₂, from ih₂ (P' ⋀ term.unop unop.not x) h1 h2,
 
       have FV P' ⊆ FV P, from set.subset_of_eq free_P'_P,
@@ -1653,13 +1149,13 @@ theorem preservation {s s': stack}: (⊢ₛ s) → (s ⟶ s') → (⊢ₛ s') :=
               assume σ: env,
 
               have hb1: dominates σ (R₂ ⋀ H₂ ⋀ P₃) ((H₂ ⋀ P₃) ⋀ R₂),
-              from dominates_and_symm,
+              from dominates.and_symm,
 
               have hb2: dominates σ ((H₂ ⋀ P₃) ⋀ R₂) (H₂ ⋀ P₃ ⋀ R₂),
-              from dominates_and_rcomm,
+              from dominates.and_assoc.symm,
 
               have hb3: dominates σ (↑H₂ ⋀ P₃ ⋀ ↑R₂) ((P₃ ⋀ ↑R₂) ⋀ H₂),
-              from dominates_and_symm,
+              from dominates.and_symm,
 
               have hb4: dominates σ (P₃ ⋀ ↑R₂) (Q₂ ⋀ spec.func g gx R₂ S₂ ⋀ R₂), from (
 
@@ -1675,20 +1171,20 @@ theorem preservation {s s': stack}: (⊢ₛ s) → (s ⟶ s') → (⊢ₛ s') :=
                 from dominates.trans hb3 this,
 
                 have hb8: dominates σ (P₃ ⋀ ↑R₂) ((Q₂ ⋀ spec.func g gx R₂ S₂) ⋀ R₂),
-                from dominates_and_left this,
+                from dominates.same_right (λ_, this),
 
                 have hb9: dominates σ ((Q₂ ⋀ spec.func g gx R₂ S₂) ⋀ R₂) (Q₂ ⋀ spec.func g gx R₂ S₂ ⋀ R₂),
-                from dominates_and_rcomm,
+                from dominates.and_assoc.symm,
 
                 show dominates σ (P₃ ⋀ ↑R₂) (Q₂ ⋀ spec.func g gx R₂ S₂ ⋀ R₂),
                 from dominates.trans hb8 hb9
               ),
 
               have hb5: dominates σ ((P₃ ⋀ ↑R₂) ⋀ H₂) ((Q₂ ⋀ spec.func g gx R₂ S₂ ⋀ R₂) ⋀ H₂),
-              from dominates_and_left hb4,
+              from dominates.same_right (λ_, hb4),
 
               have hb6: dominates σ ((Q₂ ⋀ spec.func g gx R₂ S₂ ⋀ R₂) ⋀ H₂) (↑H₂ ⋀ Q₂ ⋀ spec.func g gx R₂ S₂ ⋀ R₂),
-              from dominates_and_symm,
+              from dominates.and_symm,
 
               show dominates σ (R₂ ⋀ H₂ ⋀ P₃) (H₂ ⋀ Q₂ ⋀ spec.func g gx R₂ S₂ ⋀ R₂),
               from dominates.trans (dominates.trans (dominates.trans (dominates.trans hb1 hb2) hb3) hb5) hb6
@@ -1745,23 +1241,23 @@ theorem preservation {s s': stack}: (⊢ₛ s) → (s ⟶ s') → (⊢ₛ s') :=
 
               have haa1: dominates σ (↑H ⋀ P ⋀ prop.call f x ⋀ prop.post f x ⋀ y ≡ term.app f x)
                                ((↑H ⋀ P) ⋀ prop.call f x ⋀ prop.post f x ⋀ y ≡ term.app f x),
-              from dominates_and_comm,
+              from dominates.and_assoc,
 
               have haa2: dominates σ (↑R ⋀ ↑H ⋀ P ⋀ prop.call f x ⋀ prop.post f x ⋀ y ≡ term.app f x)
                                      ((↑H ⋀ P ⋀ prop.call f x ⋀ prop.post f x ⋀ y ≡ term.app f x) ⋀ ↑R),
-              from dominates_and_symm,
+              from dominates.and_symm,
 
               have haa3: dominates σ ((↑H ⋀ P ⋀ prop.call f x ⋀ prop.post f x ⋀ y ≡ term.app f x) ⋀ ↑R)
                                      (((↑H ⋀ P) ⋀ prop.call f x ⋀ prop.post f x ⋀ y ≡ term.app f x) ⋀ ↑ R),
-              from dominates_and_left haa1,
+              from dominates.same_right (λ_, haa1),
 
               have haa4: dominates σ (((↑H ⋀ P) ⋀ prop.call f x ⋀ prop.post f x ⋀ y ≡ term.app f x) ⋀ ↑R)
                                      (↑R ⋀ (↑H ⋀ P) ⋀ prop.call f x ⋀ prop.post f x ⋀ y ≡ term.app f x),
-              from dominates_and_symm,
+              from dominates.and_symm,
               
               have haa5: dominates σ (↑R ⋀ (↑H ⋀ P) ⋀ prop.call f x ⋀ prop.post f x ⋀ y ≡ term.app f x)
                                      ((↑R ⋀ (↑H ⋀ P)) ⋀ prop.call f x ⋀ prop.post f x ⋀ y ≡ term.app f x),
-              from dominates_and_comm,
+              from dominates.and_assoc,
               
               show dominates σ (↑R ⋀ ↑H ⋀ P ⋀ prop.call f x ⋀ prop.post f x ⋀ y ≡ term.app f x)
                                ((↑R ⋀ (↑H ⋀ P)) ⋀ prop.call f x ⋀ prop.post f x ⋀ y ≡ term.app f x),
@@ -1773,7 +1269,7 @@ theorem preservation {s s': stack}: (⊢ₛ s) → (s ⟶ s') → (⊢ₛ s') :=
 
           have h8: ⟪ prop.implies (↑R ⋀ ↑H ⋀ P ⋀ prop.call f x) (↑(term.unop unop.isFunc f) ⋀ prop.pre f x) ⟫, from (
             assume σ: env,
-            have ha1: dominates σ (↑R ⋀ ↑H ⋀ P ⋀ prop.call f x) ((↑R ⋀ ↑H ⋀ P) ⋀ prop.call f x), from dominates_shuffle,
+            have ha1: dominates σ (↑R ⋀ ↑H ⋀ P ⋀ prop.call f x) ((↑R ⋀ ↑H ⋀ P) ⋀ prop.call f x), from dominates.shuffle,
 
             have ha2: FV (↑R ⋀ ↑H ⋀ P ⋀ prop.call f x) ⊆ FV ((↑R ⋀ ↑H ⋀ P) ⋀ prop.call f x), from (
               assume z: var,
